\chapter{Kernel Extraction}
\label{chap:kernel-extraction}


\subsection{Flattening Example and Rules}
\label{subsec:kernel-extraction}

\begin{figure}
\begin{subfigure}{0.48\columnwidth}
\begin{lstlisting}
let (asss, bss) =
map
   (\ps: ([m][m]int,[m]int) ->
    let ass =
    map (\p: [m]int ->
        @let cs =@
        @  scan (+) 0 (iota p)@
        @let r = reduce (+) 0 cs@
        let as = map (+r) ps
        in as)
      ps
    let bs =
    @loop (ws=ps) for i < n do@
        let ws' =
        map (\as w: int ->
            let d = reduce (+) 0 as
            let e = d + w
            let w' = 2 * e
             in w')
          ass ws
        in ws'
    in (ass, bs))
  pss -- pss : [m][m]int
\end{lstlisting}
\caption{Program before distribution.}
\label{fig:before-distrib}
\end{subfigure}
\begin{subfigure}{0.49\columnwidth}
\begin{lstlisting}
let rss =
map (\ps: [m]int ->
    map (\p: int ->
      @let cs = scan (+) 0 (iota p)@
      @let r = reduce (+) 0 cs@
      in r)
    ps) pss
let asss =
map (\ps rs: [m]int ->
      map (\int (r) ->
         map (+r) ps)
       fs) pss rss
let bss =
@loop (wss=pss) for i < n do@
    let dss =
      map(\ass: [m]int ->
          map(\as: int ->
              reduce (+) 0 as
        , ass), asss) in
      map (\ws, ds: [m]int ->
          map (\w d: int ->
              let e = d + w in
              let w' = 2 * e in w')
          ws ds) wss dss
\end{lstlisting}
\caption{Program after distribution.}
\label{fig:after-result}
\end{subfigure}
\caption{Extracting kernels from a complicated nesting.}
\end{figure}



\begin{figure}
\small
\begin{align*}
\inference{
\Sigma \vd \Map~\Par{\fn~\overline{x}~\rightarrow~e}~\overline{y} \Rightarrow e'
}{
\Sigma, \M~\overline{x}~\overline{y} \vd e \Rightarrow e'
}
\tagsc{G1}
\end{align*}

\begin{align*}
\inference{
\Sigma, \M~\overline{x}~\overline{y} \vd e \Rightarrow e'
}{
\Sigma \vd \Map~\Par{\fn~\overline{x}~\rightarrow~e}~\overline{y} \Rightarrow e'
}
\tagsc{G2}
\end{align*}

\begin{align*}
\inference{
}{
\emptyset \vd e \Rightarrow e
}
\tagsc{G3}
\end{align*}

\begin{align*}
\inference{
  \Sigma = \Mv{x_p}{y_p},\ldots,\Mv{x_1}{y_1} \\
  \Sigma' = \M~(\ov{x_p},\ov{a_{p-1}})~(\ov{y_p}, \ov{a_{p}}), \ldots, \M~(\ov{x_1},\ov{a_{0}})~(\ov{y_1},\ov{a_{1}}^{q_1}) \\
  \overline{a_{p}}, \dots, \overline{a_{1}} ~\mbox{fresh~names} \\
  \mbox{size~of~each~array~in~}\overline{a_{0}}\mbox{~invariant~to~}\Sigma \\
  \Sigma \vd e_1 \Rightarrow e_1' ~~~~ \Sigma' \vd e_2 \Rightarrow e_2'
}{
\Sigma \vd \Let~\ov{a_0} ~\kt{=}~e_1~\kw{in}~e_2 \Rightarrow \Let~\ov{a_p}~\kt{=}~ e_1' ~\kw{in}~e_2'
}
\tagsc{G4}
\end{align*}

\begin{align*}
\inference{
  g = \Reduce~\Par{\fn~\ov{y}^{2*p} ~\rightarrow ~e}~\ov{n}^p \\
  \Sigma \vd \Map~\Par{g} ~\Par{\Transpose~z_0}\ldots\Par{\Transpose~z_{p-1}} \Rightarrow e' \\
  f = \Map~\Par{\fn~\ov{y}^{2*p}~\rightarrow e}
}{
\Sigma \vd \Reduce~\Par{f}~\Par{\ov{\Replicate~k ~n}^p}~\ov{z}^p \Rightarrow e'
}
\tagsc{G5}
\end{align*}

\begin{align*}
\inference{
\Sigma \vd \Rearrange~\Par{0,1+k_0,\ldots,1+k_{n-1}}~y \Rightarrow e
}{
\Sigma, \M~x~y \vd \Rearrange~\overline{k}^n ~ x \Rightarrow e
}
\tagsc{G6}
\end{align*}

\begin{align*}
\inference{
  \Sigma' = \Sigma, \M~(\ov{x},\ov{y})~(\ov{xs},\ov{ys}) \hspace{1.2cm} (\{n\}\cup\ov{q}) \cap (\ov{x},\ov{y}) = \emptyset \\
  m = \mbox{outer~size~of~each~of~} \ov{xs} \mbox{~and~} \ov{ys}\\
  \mbox{f~contains~exploitable~(regular)~inner~parallelism}\\
  \Sigma \vd \Loop~\Par{\ov{zs'}~\kt{=}~\ov{\Replicate~m~z_i}, \ov{ys'}~\kt{=}~\ov{ys}} \\
    \hspace{1.8cm}\For~ i~\kt{<}~n~ \Do~\Map \Par{f~i~\ov{q}} ~\ov{xs}~\ov{ys}~\ov{ys'}~\ov{zs'} \Rightarrow e
}{
  \Sigma' \vd \begin{array}[t]{l} \Loop~\Par{\ov{z'}~\kt{=}~\ov{z},~\ov{y'}~\kt{=}~\ov{y}}~\kt{=}~ \\
  ~~ \For~i~\kt{<}~n~ \Do~ f~i~\ov{q}~\ov{x}~\ov{y}~\ov{y'}~\ov{z} \Rightarrow e \end{array}
}
\tagsc{G7}
\end{align*}
\caption{Flattening rules.}
\label{fig:flattening-rules}
\end{figure}


%%% Local Variables:
%%% mode: latex
%%% TeX-master: "thesis"
%%% End:
